---
title: "K-th Symbol in Grammar"
layout: post
date: 2021-08-01 01:11:37
image: /assets/images/logo_leetcode.png
headerImage: false
tag:
- github pages
- blog
category: blog
author: chaeeon-lim
description: Problem description and solution 
---

We build a table of `n` rows (**1-indexed**). We start by writing `0` in the `1st` row. Now in every subsequent row, we look at the previous row and replace each occurrence of `0` with `01`, and each occurrence of `1` with `10`.

* For example, for n = 3, the 1st row is 0, the 2nd row is 01, and the 3rd row is 0110.

Given two integer n and k, return the kth (**1-indexed**) symbol in the nth row of a table of n rows.

```python
class Solution:
    def recursion(self, n, k):
        if n == 1:
            return 0

        prevN = n-1
        if k <= 2**(n-2):
            return self.recursion(prevN, k)
        else:
            return (self.recursion(prevN, (k-2**(n-2)))+1)%2

    def kthGrammar(self, n: int, k: int) -> int:
        result = 0
        return result
```


(1,1) = 0
(2,1) =  (1,1) = 0
(2,2) = ~(1,1) = 1
(3,1) =  (2,1) =  (1,1) = 0
(3,2) =  (2,2) = ~(1,1) = 1
(3,3) = ~(2,1) = ~(1,1) = 1
(3,4) = ~(2,2) =  (1,1) = 0

(4,1) =   (3,1) =  (2,1) =  (1,1) = 0
(4,2) =   (3,2) =  (2,2) = ~(1,1) = 1
(4,3) =   (3,3) = ~(2,1) = ~(1,1) = 1
(4,4) =   (3,4) = ~(2,2) =  (1,1) = 0
(4,5) =  ~(3,1) = ~(2,1) = ~(1,1) = 0
(4,6) =  ~(3,2) = ~(2,2) =  (1,1) = 1
(4,7) =  ~(3,3) =  (2,1) =  (1,1) = 1
(4,8) =  ~(3,4) =  (2,2) = ~(1,1) = 0
